New logrel

theories/Dot/lr/unary_lr.v
@@ -34,7 +34,8 @@ Notation "Ds⟦ T ⟧" := (clty_dslty C⟦ T ⟧).
 (* We could inline [pty_interp] inside the [V⟦ _ ⟧] notation, but I suspect
 the [V⟦ _ ⟧*] notation needs [pty_interp] to be a first-class function. *)
 Definition pty_interp `{CTyInterp Σ} T : oltyO Σ := clty_olty C⟦ T ⟧.
-#[global] Arguments pty_interp {_ _} !_ /.
+(* #[global] Arguments pty_interp {_ _} !_ /. *)
+#[global] Arguments pty_interp : simpl never.
 
 (** * Value interpretation of types (Fig. 9). *)
 Notation "V⟦ T ⟧" := (pty_interp T).
@@ -122,18 +123,22 @@ Section log_rel.
   (* Observe the naming pattern for semantic type constructors:
   replace T by o (for most constructors) or by c (for constructors producing
   cltys). *)
-  Fixpoint kind_interp (K : kind) : sf_kind Σ :=
-    let rec_ty := ty_interp : CTyInterp Σ in
-    let rec_kind := kind_interp : SfKindInterp Σ in
+  Implicit Type (hrec : ty -d> hoEnvD Σ).
+  Implicit Type (clrec : ty -d> cltyO Σ).
+
+  Fixpoint kind_rec clrec (K : kind) {struct K} : sf_kind Σ :=
+    let rec_ty := ty_rec clrec : CTyInterp Σ in
+    let rec_kind := kind_rec clrec : SfKindInterp Σ in
     match K with
     | kintv L U => sf_kintv V⟦ L ⟧ V⟦ U ⟧
     | kpi S K => sf_kpi V⟦ S ⟧ K⟦ K ⟧
     end
-   with ty_interp (T : ty) : clty Σ :=
-    let rec_ty := ty_interp : CTyInterp Σ in
-    let rec_kind := kind_interp : SfKindInterp Σ in
+   with ty_rec clrec (T : ty) {struct T} : clty Σ :=
+    let rec_ty := ty_rec clrec : CTyInterp Σ in
+    let rec_kind := kind_rec clrec : SfKindInterp Σ in
+    let hrec T := clty_olty $ clrec T in
     match T with
-    | kTTMem l K => cTMemK l K⟦ K ⟧
+    | kTTMem l K => cTMemK l hrec K⟦ K ⟧
     | TVMem l T' => cVMem l V⟦ T' ⟧
     | TAnd T1 T2 => cAnd C⟦ T1 ⟧ C⟦ T2 ⟧
     | TTop => cTop
@@ -145,19 +150,159 @@ Section log_rel.
     | TPrim b => olty2clty $ oPrim b
     | TAll T1 T2 => olty2clty $ oAll V⟦ T1 ⟧ V⟦ T2 ⟧
     | TMu T => olty2clty $ oMu V⟦ T ⟧
-    | kTSel n p l => olty2clty $ oSel p l
+    | kTSel n p l => olty2clty $ oSel p l hrec
     | TSing p => olty2clty $ oSing p
     | TLam T => olty2clty $ oLam V⟦ T ⟧
     | TApp T p => olty2clty $ oTApp V⟦ T ⟧ p
     end.
 
-  #[global] Instance dot_ty_interp : CTyInterp Σ := Reduce ty_interp.
-  #[global] Instance dot_kind_interp : SfKindInterp Σ := Reduce kind_interp.
+  (* Notation Contractive2 f := (∀ n, Proper (dist_later n ==> dist_later n ==> dist n) f). *)
+  Section interp_contractive.
+    Context (ri1 ri2 : ty -d> cltyO Σ).
 
+    Lemma interp_contractive_mut n (Hri : dist_later n ri1 ri2) :
+      (∀ T, ty_rec ri1 T ≡{n}≡ ty_rec ri2 T) ∧
+      (∀ K, kind_rec ri1 K ≡{n}≡ kind_rec ri2 K).
+    Proof.
+      apply tp_kn_mut_ind; simpl; [done|done|..]; intros *.
+      all: rewrite /pty_interp/clty_interp/sf_kind_interp.
+      Time all: intros; try by repeat (hof_eq_app || f_equiv).
+      all: repeat (hof_eq_app || f_contractive || f_equiv).
+      all: intros ????; apply clty_olty_ne, Hri.
+    Qed.
+  End interp_contractive.
+
+  #[global] Instance kind_rec_contractive :
+    Contractive (kind_rec : _ -d> kind -d> sf_kindO Σ).
+  Proof. by move=> /= n ri1 ri2 Hri x; apply interp_contractive_mut. Qed.
+  #[global] Instance ty_rec_contractive :
+    Contractive (ty_rec : _ -d> ty -d> cltyO Σ).
+  Proof. by move=> /= n ri1 ri2 Hri x; apply interp_contractive_mut. Qed.
+
+  #[global] Instance ty_interp : CTyInterp Σ := fixpoint ty_rec.
+  #[global] Arguments clty_interp {_ _} _ : simpl never.
+  #[global] Instance dot_kind_interp : SfKindInterp Σ := kind_rec ty_interp.
+  #[global] Arguments sf_kind_interp {_ _} _ : simpl never.
+
+  Lemma fixpoint_interp_eq1 T : C⟦ T ⟧ ≡ ty_rec ty_interp T.
+  Proof. apply: fixpoint_unfold. Qed.
+  Ltac rewrite_interp := repeat (rewrite fixpoint_interp_eq1 //=; repeat f_equiv).
+  Lemma fixpoint_interp_eq : ty_interp ≡@{ty -d> _} ty_rec ty_interp.
+  Proof. apply: fixpoint_unfold. Qed.
+  #[global] Instance kind_rec_ne :
+    NonExpansive (kind_rec : _ -d> kind -d> sf_kindO Σ) := _.
+  #[global] Instance kind_rec_proper :
+    Proper1 (kind_rec : _ -d> kind -d> sf_kindO Σ) := _.
+
+  Lemma krec_unfold0 : kind_rec (ty_rec ty_interp) ≡@{kind -d> sf_kindO Σ} kind_rec ty_interp.
+  Proof. by rewrite /sf_kind_interp/dot_kind_interp -fixpoint_unfold. Qed.
+  Lemma krec_unfold K : K⟦ K ⟧ ≡ kind_rec ty_interp K.
+  Proof. done. Qed.
+  Lemma trec_fold0 : ty_rec ty_interp ≡@{ty -d> cltyO Σ} ty_interp.
+  Proof. apply symmetry, fixpoint_unfold. Qed.
+
+  Lemma kinterp_kintv L U : K⟦ kintv L U ⟧ ≡ sf_kintv V⟦ L ⟧ V⟦ U ⟧.
+  Proof. apply sf_kintv_proper; apply trec_fold0. Qed.
+  Lemma kinterp_kpi S K : K⟦ kpi S K ⟧ ≡ sf_kpi V⟦ S ⟧ K⟦ K ⟧.
+  Proof. apply sf_kpi_proper. apply trec_fold0. done. Qed.
+  Definition klr := (kinterp_kintv, kinterp_kpi).
+  Ltac kgo := rewrite ?klr.
+
+    (* | kintv L U => sf_kintv V⟦ L ⟧ V⟦ U ⟧
+    | kpi S K => sf_kpi V⟦ S ⟧ K⟦ K ⟧ *)
+
+  Notation cBot := (olty2clty oBot).
+  Notation cOr T1 T2 := (olty2clty $ oOr T1 T2).
+  Notation cLater T := (olty2clty $ oLater T).
+  Notation cPrim b := (olty2clty $ oPrim b).
+  Notation cAll T1 T2 := (olty2clty $ oAll T1 T2).
+  Notation cMu T := (olty2clty $ oMu T).
+  Notation cSel p l pty := (olty2clty $ oSel p l pty).
+  Notation cSing p := (olty2clty $ oSing p).
+  Notation cLam T := (olty2clty $ oLam T).
+  Notation cApp T p := (olty2clty $ oTApp T p).
+
+  (* #[global] Arguments sf_kind_interp {_ _} _ : simpl never. *)
+  Lemma cinterp_TTop : C⟦ TTop ⟧ ≡ cTop.
+  Proof. apply fixpoint_interp_eq1. Qed.
+  Lemma cinterp_TBot : C⟦ TBot ⟧ ≡ cBot.
+  Proof. apply fixpoint_interp_eq1. Qed.
+
+  Ltac go :=
+    rewrite fixpoint_interp_eq1 /= /pty_interp/clty_interp//=;
+    by rewrite -fixpoint_unfold.
+  Lemma cinterp_kTTMem l K1 : C⟦ kTTMem l K1 ⟧ ≡ cTMemK l pty_interp K⟦ K1 ⟧.
+  Proof. go. Qed.
+  Lemma cinterp_kTSel n p l : C⟦ kTSel n p l ⟧ ≡ cSel p l pty_interp.
+  Proof. go. Qed.
+
+  Lemma cinterp_TAnd T1 T2 : C⟦ TAnd T1 T2 ⟧ ≡ cAnd C⟦ T1 ⟧ C⟦ T2 ⟧.
+  Proof. by rewrite !fixpoint_interp_eq1. Qed.
+  (* Lemma cinterp_TAnd T1 T2 args : C⟦ TAnd T1 T2 ⟧ args ≡ cAnd C⟦ T1 ⟧ C⟦ T2 ⟧ args .
+  Proof. rewrite fixpoint_interp_eq1/=. Qed. *)
+  Lemma cinterp_TOr T1 T2 : C⟦ TOr T1 T2 ⟧ ≡ cOr V⟦ T1 ⟧ V⟦ T2 ⟧.
+  Proof. go. Qed.
+  Lemma cinterp_TLater T1 : C⟦ TLater T1 ⟧ ≡ cLater V⟦ T1 ⟧.
+  Proof. go. Qed.
+  Lemma cinterp_TAll T1 T2 : C⟦ TAll T1 T2 ⟧ ≡ cAll V⟦ T1 ⟧ V⟦ T2 ⟧.
+  Proof. go. Qed.
+  Lemma cinterp_TMu T1 : C⟦ TMu T1 ⟧ ≡ cMu V⟦ T1 ⟧.
+  Proof. go. Qed.
+  Lemma cinterp_TVMem l T1 : C⟦ TVMem l T1 ⟧ ≡ cVMem l V⟦ T1 ⟧.
+  Proof. go. Qed.
+  Lemma cinterp_TPrim b : C⟦ TPrim b ⟧ ≡ cPrim b.
+  Proof. apply fixpoint_interp_eq1. Qed.
+  Lemma cinterp_TSing p : C⟦ TSing p ⟧ ≡ cSing p.
+  Proof. apply fixpoint_interp_eq1. Qed.
+  Lemma cinterp_TLam T1 : C⟦ TLam T1 ⟧ ≡ cLam V⟦ T1 ⟧.
+  Proof. go. Qed.
+  Lemma cinterp_TApp T1 p : C⟦ TApp T1 p ⟧ ≡ cApp V⟦ T1 ⟧ p.
+  Proof. go. Qed.
+  Definition clr :=
+    (cinterp_TTop, cinterp_TBot, cinterp_TAnd,
+    cinterp_TOr, cinterp_TLater, cinterp_TAll, cinterp_TMu, cinterp_TVMem,
+    cinterp_kTTMem, cinterp_kTSel, cinterp_TPrim, cinterp_TSing, cinterp_TLam, cinterp_TApp).
+
+  Ltac go ::= rewrite /pty_interp clr //.
+
+  Lemma interp_TTop : V⟦ TTop ⟧ ≡ oTop.
+  Proof. go. Qed.
+  Lemma interp_TBot : V⟦ TBot ⟧ ≡ oBot.
+  Proof. go. Qed.
+  Lemma interp_TAnd T1 T2 : V⟦ TAnd T1 T2 ⟧ ≡ oAnd V⟦ T1 ⟧ V⟦ T2 ⟧.
+  Proof. go. Qed.
+  Lemma interp_TOr T1 T2 : V⟦ TOr T1 T2 ⟧ ≡ oOr V⟦ T1 ⟧ V⟦ T2 ⟧.
+  Proof. go. Qed.
+  Lemma interp_TLater T1 : V⟦ TLater T1 ⟧ ≡ oLater V⟦ T1 ⟧.
+  Proof. go. Qed.
+  Lemma interp_TAll T1 T2 : V⟦ TAll T1 T2 ⟧ ≡ oAll V⟦ T1 ⟧ V⟦ T2 ⟧.
+  Proof. go. Qed.
+  Lemma interp_TMu T1 : V⟦ TMu T1 ⟧ ≡ oMu V⟦ T1 ⟧.
+  Proof. go. Qed.
+  Lemma interp_TVMem l T1 : V⟦ TVMem l T1 ⟧ ≡ oVMem l V⟦ T1 ⟧.
+  Proof. go. Qed.
+  Lemma interp_kTTMem l K1 : V⟦ kTTMem l K1 ⟧ ≡ oTMemK l pty_interp K⟦ K1 ⟧.
+  Proof. go. Qed.
+  Lemma interp_kTSel n p l : V⟦ kTSel n p l ⟧ ≡ oSel p l pty_interp.
+  Proof. go. Qed.
+  Lemma interp_TPrim b : V⟦ TPrim b ⟧ ≡ oPrim b.
+  Proof. go. Qed.
+  Lemma interp_TSing p : V⟦ TSing p ⟧ ≡ oSing p.
+  Proof. go. Qed.
+  Lemma interp_TLam T1 : V⟦ TLam T1 ⟧ ≡ oLam V⟦ T1 ⟧.
+  Proof. go. Qed.
+  Lemma interp_TApp T1 p : V⟦ TApp T1 p ⟧ ≡ oTApp V⟦ T1 ⟧ p.
+  Proof. go. Qed.
   (** Unfolding lemma for [TAnd]: defined because [simpl] on the LHS produces
       [oAnd C⟦ T1 ⟧ C⟦ T2 ⟧]. *)
   Lemma interp_TAnd_eq T1 T2 : V⟦ TAnd T1 T2 ⟧ ≡ oAnd V⟦ T1 ⟧ V⟦ T2 ⟧.
-  Proof. done. Qed.
+  Proof. apply interp_TAnd. Qed.
+
+  Definition vlr :=
+    (interp_TTop, interp_TBot, interp_TAnd,
+    interp_TOr, interp_TLater, interp_TAll, interp_TMu, interp_TVMem,
+    interp_kTTMem, interp_kTSel, interp_TPrim, interp_TSing, interp_TLam, interp_TApp).
+  Ltac vgo := rewrite ?vlr.
 
   (** Binding lemmas for [V⟦ T ⟧] and [K⟦ T ⟧]. *)
   Lemma mut_interp_subst_compose_ind :
@@ -166,11 +311,60 @@ Section log_rel.
     (∀ K ρ1 ρ2 τ1 τ2,
       K⟦ K.|[ρ1] ⟧ ρ2 τ1 τ2 ⊣⊢ K⟦ K ⟧ (ρ1 >> ρ2) τ1 τ2).
   Proof.
-    rewrite /pty_interp; apply tp_kn_mut_ind; intros;
-      rewrite /= /pty_interp /sr_kintv /subtype_lty; properness;
+    apply tp_kn_mut_ind; intros; vgo; kgo;
+      rewrite /= /sr_kintv /subtype_lty; properness;
+      rewrite ?scons_up_swap ?hsubst_comp; trivial.
+    all: try by apply path_wp_proper => ?.
+  Qed.
+  (*
+  Lemma vrec3 T args ρ v : V⟦ T ⟧ args ρ v ≡ ty_rec ty_interp T.
+  Proof. apply: fixpoint_unfold. Qed.
+    rewrite trec_fold0.
+    eapply H.
+    apply H.
+    rewrite /pty_interp/clty_interp.
+    f_equiv.
+    Fail rewrite -fixpoint_interp_eq1.
+    Fail rewrite fixpoint_unfold.
+    Fail rewrite -fixpoint_unfold.
+    all: unfold pty_interp in *.
+    rewrite krec_unfold.
+    f_equiv.
+      rewrite ?scons_up_swap ?hsubst_comp; trivial.
+    apply clty_o
+      rewrite -fixpoint_interp_eq1. ixpoint_unfold.
+    all: vgo.
+
+
+
+    apply tp_kn_mut_ind; intros.
+    all: vgo.
+
+    all: rewrite /= /sr_kintv /subtype_lty;
+      properness;
+      rewrite ?scons_up_swap ?hsubst_comp; trivial.
+    all: try by apply path_wp_proper => ?.
+    rewrite /pty_interp.
+    f_equiv.
+      rewrite ?scons_up_swap ?hsubst_comp; trivial.
+    apply clty_o
+      rewrite -fixpoint_interp_eq1. ixpoint_unfold.
+    all: vgo.
+
+
+    rewrite /sr_kintv /subtype_lty. vgo; simpl.
+
+    apply H.
+    trivial.
+    rewrite /pty_interp; apply tp_kn_mut_ind; intros.
+    simpl.
+
+      rewrite /= /pty_interp.
+      eapply clty_olty_proper.
+      rewrite ?clr. /sr_kintv /subtype_lty; properness;
       rewrite ?scons_up_swap ?hsubst_comp; trivial.
     all: by apply path_wp_proper => ?.
-  Qed.
+  Qed. *)
 
   #[global] Instance pinterp_lemmas: CTyInterpLemmas Σ.
   Proof. split. apply mut_interp_subst_compose_ind. Qed.
@@ -226,7 +420,7 @@ Section misc_lemmas.
 
   Lemma iterate_TLater_oLater i (T : ty) :
     V⟦iterate TLater i T⟧ ≡ oLaterN i V⟦T⟧.
-  Proof. elim: i => [//|i IHi] ???; by rewrite !iterate_S /= IHi. Qed.
+  Proof. elim: i => [//|i IHi] ???. by rewrite !iterate_S vlr /= IHi. Qed.
 
 End misc_lemmas.
 
@@ -243,8 +437,9 @@ Section path_repl_lemmas.
   Proof.
     apply ty_kind_path_repl_mut_ind;
     rewrite /fundamental_ty_path_repl_def /fundamental_kn_path_repl_def
-      /sem_ty_path_repl /sem_kind_path_repl; cbn;
-      rewrite /pty_interp /sr_kintv /subtype_lty/=; intros;
+      /sem_ty_path_repl /sem_kind_path_repl; intros.
+      all: rewrite ?vlr ?klr /=.
+      all: rewrite /sr_kintv /subtype_lty/=; intros;
       try match goal with
       | H : context [equiv _ _] |- _ => rename H into IHHrew
       end;
@@ -305,8 +500,8 @@ End path_repl_lemmas.
 (** Backward compatibility. *)
 Notation "⟦ T ⟧" := (oClose V⟦ T ⟧).
 
-Definition lr := (@fmap_cons, @iterate_TLater_oLater).
-Ltac rw := rewrite /ietp /idstp /idtp /iptp /istpd ?lr /=.
+Definition lr := (@fmap_cons, @iterate_TLater_oLater, @vlr, @klr, @clr).
+Ltac rw := rewrite /ietp /idstp /idtp /iptp /istpd ?lr.
 
 Import dlang_adequacy.
 
